cfrontend/BeePL_typechecker.v
@@ -1,6 +1,6 @@
 Require Import String ZArith Coq.FSets.FMapAVL Coq.Structures.OrderedTypeEx Coq.Strings.BinaryString.
 Require Import Coq.FSets.FSetProperties Coq.FSets.FMapFacts FMaps FSetAVL Nat PeanoNat Coq.Lists.List.
-Require Import Coq.Arith.EqNat Coq.ZArith.Int Integers AST Maps Ctypes.
+Require Import Coq.Arith.EqNat Coq.ZArith.Int Integers AST Maps Ctypes Ctyping.
 Require Import BeePL_aux BeePL BeePL_values BeeTypes BeePL_mem Errors.
 From mathcomp Require Import all_ssreflect. 
 
@@ -31,14 +31,46 @@ match v with
 | Vloc p ofs => Twptr
 end.
 
-Section Type_check_exprs.
-Variable type_check_expr : ty_context -> store_context -> expr -> res (type * effect).
+Section Trans_ctypes_btypes.
 
-Fixpoint type_check_exprs (Gamma : ty_context) (Sigma : store_context) (es : list expr) : res (list type * effect) :=
+Variable trans_ctype_btype : Ctypes.type -> res BeeTypes.type.
+
+Fixpoint trans_ctypes_btypes (ct : typelist) : res (list BeeTypes.type) :=
+match ct with 
+| Tnil => OK nil
+| Tcons ct cts => do bt <- trans_ctype_btype ct;
+                  do bts <- trans_ctypes_btypes cts;
+                  OK (bt :: bts)
+end.
+
+End Trans_ctypes_btypes.
+
+Definition trans_ctype_btype (ct : Ctypes.type) : res BeeTypes.type :=
+match ct with 
+| Tvoid => OK (Ptype Tunit)
+| Ctypes.Tint sz s a => OK (BeeTypes.Ptype (Tint sz s a))
+| Ctypes.Tlong s a => OK (BeeTypes.Ptype (Tlong s a))
+| Tfloat _ _ => Error (msg "Float is not supported in BeePL")
+| Tpointer t a => match t with 
+                  | Tvoid => OK (Reftype 1%positive (Bprim Tunit) a)
+                  | Ctypes.Tint sz s a => OK (Reftype 1%positive (Bprim (Tint sz s a)) a)
+                  | Ctypes.Tlong s a => OK (Reftype 1%positive (Bprim (Tlong s a)) a)
+                  | _ => Error (msg "Not supported in ref type")
+                  end 
+| Tarray t z a => Error (msg "Array is not supported in BeePL")
+| Tfunction ts t cc => Error (msg "Cannot compute the effect, hence translation is not possible from ctype to btype in case of function")
+| Tstruct x a => OK (Stype x a)
+| Tunion x a => Error (msg "Union is not supported in BeePL")
+end.
+
+Section Type_check_exprs.
+Variable type_check_expr : bcomposite_env -> ty_context -> store_context -> expr -> res (type * effect).
+
+Fixpoint type_check_exprs (cenv : bcomposite_env) (Gamma : ty_context) (Sigma : store_context) (es : list expr) : res (list type * effect) :=
 match es with 
 | nil => OK (nil, nil)
-| e :: es => do (te, efe) <- type_check_expr Gamma Sigma e;
-             do (tes, efes) <- type_check_exprs Gamma Sigma es;
+| e :: es => do (te, efe) <- type_check_expr cenv Gamma Sigma e;
+             do (tes, efes) <- type_check_exprs cenv Gamma Sigma es;
              OK (te :: tes, efe ++ efes)
 end.
 
@@ -46,7 +78,7 @@ End Type_check_exprs.
 
 Definition mem_ident := 2%positive.
 
-Fixpoint type_check_expr (Gamma : ty_context) (Sigma : store_context) (e : expr) : res (type * effect) :=
+Fixpoint type_check_expr (cenv : bcomposite_env) (Gamma : ty_context) (Sigma : store_context) (e : expr) : res (type * effect) :=
 match e with 
 | Val v t => OK (t, nil)
 | Var x t => match (PTree.get x (extend_context Gamma x t)) with 
@@ -54,8 +86,8 @@ match e with
              | None => Error (msg "Variable not found")
              end
 | Const c t => OK (t, nil)
-| App e es t => do (ft, efe) <- type_check_expr Gamma Sigma e;
-                do (ts, efs) <- type_check_exprs type_check_expr Gamma Sigma es;
+| App e es t => do (ft, efe) <- type_check_expr cenv Gamma Sigma e;
+                do (ts, efs) <- type_check_exprs type_check_expr cenv Gamma Sigma es;
                 match ft with 
                 | Ftype ts1 ef rt1 => if eq_types eq_type ts ts1 && eq_type rt1 t
                                       then OK (rt1, efe ++ ef ++ efs) 
@@ -64,7 +96,7 @@ match e with
                 end
 | Prim b es t => match b with 
                  | Ref => match es with 
-                          | e :: nil => do (te, ef) <- type_check_expr Gamma Sigma e;
+                          | e :: nil => do (te, ef) <- type_check_expr cenv Gamma Sigma e;
                                         match te with 
                                         | Ptype bt => if eq_type t (Reftype mem_ident (Bprim bt) (attr_of_primitive_type bt)) 
                                                       then OK (Reftype mem_ident (Bprim bt) (attr_of_primitive_type bt), (ef ++ (Alloc mem_ident :: nil)))
@@ -74,7 +106,7 @@ match e with
                           |  _ => Error (msg "Wrong number of arguments to Ref")
                           end
                  | Deref => match es with 
-                            | e :: nil => do (te, ef) <- type_check_expr Gamma Sigma e;
+                            | e :: nil => do (te, ef) <- type_check_expr cenv Gamma Sigma e;
                                           match te with 
                                           | Reftype mem_ident (Bprim bt) a => if eq_type t (Ptype bt) 
                                                                               then OK (Ptype bt, (ef ++ (Read mem_ident :: nil)))
@@ -84,9 +116,9 @@ match e with
                           |  _ => Error (msg "Wrong number of arguments to Deref")
                           end
                  | Massgn => match es with 
-                             | e1 :: e2 :: nil => do (te1, ef1) <- type_check_expr Gamma Sigma e1;
+                             | e1 :: e2 :: nil => do (te1, ef1) <- type_check_expr cenv Gamma Sigma e1;
                                                   match te1 with 
-                                                  | Reftype mem_ident (Bprim bt) a => do (te2, ef2) <- type_check_expr Gamma Sigma e2;
+                                                  | Reftype mem_ident (Bprim bt) a => do (te2, ef2) <- type_check_expr cenv Gamma Sigma e2;
                                                                                       match te2 with 
                                                                                       | Ptype bt => if eq_type t (Ptype Tunit)
                                                                                                     then OK (Ptype Tunit, ef1 ++ ef2 ++ (Write mem_ident :: nil))
@@ -99,21 +131,21 @@ match e with
                             end                                                         
                  | Uop o => match o with 
                             | Cop.Onotbool => match es with 
-                                              | e :: nil => do (te, ef) <- type_check_expr Gamma Sigma e;
+                                              | e :: nil => do (te, ef) <- type_check_expr cenv Gamma Sigma e;
                                                             if is_primbool te && eq_type t te
                                                             then OK (te, ef)
                                                             else Error (msg "Wrong argument type to negation bool operator, it expects bool as argument")
                                               | _ => Error (msg "Wrong number of arguments to Unary operator")
                                               end
                             | Cop.Onotint => match es with 
-                                              | e :: nil => do (te, ef) <- type_check_expr Gamma Sigma e;
+                                              | e :: nil => do (te, ef) <- type_check_expr cenv Gamma Sigma e;
                                                             if (is_primint te || is_primlong te) && eq_type t te
                                                             then OK (te, ef)
                                                             else Error (msg "Wrong argument type to bitwise not operator, it expects int or long as argument")
                                               | _ => Error (msg "Wrong number of arguments to Unary operator")
                                               end
                             | Cop.Oneg => match es with 
-                                          | e :: nil => do (te, ef) <- type_check_expr Gamma Sigma e;
+                                          | e :: nil => do (te, ef) <- type_check_expr cenv Gamma Sigma e;
                                                         if (is_primint te || is_primlong te) && eq_type t te
                                                         then OK (te, ef)
                                                         else Error (msg "Wrong argument type to unary minus operator, it expects int or long as argument")
@@ -123,128 +155,128 @@ match e with
                             end 
                  | Bop o => match o with 
                             | Cop.Oadd => match es with 
-                                          | e1 :: e2 :: nil => do (te1, ef1) <- type_check_expr Gamma Sigma e1;
-                                                               do (te2, ef2) <- type_check_expr Gamma Sigma e2;
+                                          | e1 :: e2 :: nil => do (te1, ef1) <- type_check_expr cenv Gamma Sigma e1;
+                                                               do (te2, ef2) <- type_check_expr cenv Gamma Sigma e2;
                                                                if (eq_type te1 te2 && (is_primint te1 || is_primlong te1) && eq_effect ef1 ef2 && eq_type te1 t) 
                                                                then OK(te1, ef1)
                                                                else Error (msg "Wrong argument types to add operator, it expects int or long as argument")
                                           | _ => Error (msg "Wrong number of arguments to Binary operators") 
                                           end 
                             | Cop.Osub => match es with 
-                                          | e1 :: e2 :: nil => do (te1, ef1) <- type_check_expr Gamma Sigma e1;
-                                                               do (te2, ef2) <- type_check_expr Gamma Sigma e2;
+                                          | e1 :: e2 :: nil => do (te1, ef1) <- type_check_expr cenv Gamma Sigma e1;
+                                                               do (te2, ef2) <- type_check_expr cenv Gamma Sigma e2;
                                                                if (eq_type te1 te2 && (is_primint te1 || is_primlong te1) && eq_effect ef1 ef2 && eq_type te1 t) 
                                                                then OK(te1, ef1)
                                                                else Error (msg "Wrong argument types to add operator, it expects int or long as argument") 
                                           | _ => Error (msg "Wrong number of arguments to Binary operators") 
                                           end
                             | Cop.Omul => match es with 
-                                          | e1 :: e2 :: nil => do (te1, ef1) <- type_check_expr Gamma Sigma e1;
-                                                           do (te2, ef2) <- type_check_expr Gamma Sigma e2;
+                                          | e1 :: e2 :: nil => do (te1, ef1) <- type_check_expr cenv Gamma Sigma e1;
+                                                           do (te2, ef2) <- type_check_expr cenv Gamma Sigma e2;
                                                            if (eq_type te1 te2 && (is_primint te1 || is_primlong te1) && eq_effect ef1 ef2 && eq_type te1 t) 
                                                            then OK(te1, ef1)
                                                            else Error (msg "Wrong argument types to mul operator, it expects int or long as argument")
                                           | _ => Error (msg "Wrong number of arguments to Binary operators") 
                                           end 
                             | Cop.Odiv => match es with 
-                                          | e1 :: e2 :: nil => do (te1, ef1) <- type_check_expr Gamma Sigma e1;
-                                                           do (te2, ef2) <- type_check_expr Gamma Sigma e2;
+                                          | e1 :: e2 :: nil => do (te1, ef1) <- type_check_expr cenv Gamma Sigma e1;
+                                                           do (te2, ef2) <- type_check_expr cenv Gamma Sigma e2;
                                                            if (eq_type te1 te2 && (is_primint te1 || is_primlong te1) && eq_effect ef1 ef2 && eq_type te1 t) 
                                                            then OK(te1, ef1)
                                                            else Error (msg "Wrong argument types to div operator, it expects int or long as argument")
                                           | _ => Error (msg "Wrong number of arguments to Binary operators") 
                                           end
                             | Cop.Omod => match es with 
-                                          | e1 :: e2 :: nil => do (te1, ef1) <- type_check_expr Gamma Sigma e1;
-                                                           do (te2, ef2) <- type_check_expr Gamma Sigma e2;
+                                          | e1 :: e2 :: nil => do (te1, ef1) <- type_check_expr cenv Gamma Sigma e1;
+                                                           do (te2, ef2) <- type_check_expr cenv Gamma Sigma e2;
                                                            if (eq_type te1 te2 && (is_primint te1 || is_primlong te1) && eq_effect ef1 ef2 && eq_type te1 t) 
                                                            then OK(te1, ef1)
                                                            else Error (msg "Wrong argument types to mod operator, it expects int or long as argument") 
                                           | _ => Error (msg "Wrong number of arguments to Binary operators") 
                                           end
                             | Cop.Oand => match es with 
-                                          | e1 :: e2 :: nil => do (te1, ef1) <- type_check_expr Gamma Sigma e1;
-                                                           do (te2, ef2) <- type_check_expr Gamma Sigma e2;
+                                          | e1 :: e2 :: nil => do (te1, ef1) <- type_check_expr cenv Gamma Sigma e1;
+                                                           do (te2, ef2) <- type_check_expr cenv Gamma Sigma e2;
                                                            if (eq_type te1 te2 && (is_primint te1 || is_primlong te1) && eq_effect ef1 ef2 && eq_type te1 t) 
                                                            then OK(te1, ef1)
                                                            else Error (msg "Wrong argument types to and operator, it expects bool as argument")
                                           | _ => Error (msg "Wrong number of arguments to Binary operators") 
                                           end
                             | Cop.Oor => match es with 
-                                         | e1 :: e2 :: nil => do (te1, ef1) <- type_check_expr Gamma Sigma e1;
-                                                           do (te2, ef2) <- type_check_expr Gamma Sigma e2;
+                                         | e1 :: e2 :: nil => do (te1, ef1) <- type_check_expr cenv Gamma Sigma e1;
+                                                           do (te2, ef2) <- type_check_expr cenv Gamma Sigma e2;
                                                            if (eq_type te1 te2 && (is_primint te1 || is_primlong te1) && eq_effect ef1 ef2 && eq_type te1 t) 
                                                            then OK(te1, ef1)
                                                            else Error (msg "Wrong argument types to or operator, it expects bool as argument")
                                          | _ => Error (msg "Wrong number of arguments to Binary operators") 
                                          end
                             | Cop.Oxor => match es with 
-                                          | e1 :: e2 :: nil => do (te1, ef1) <- type_check_expr Gamma Sigma e1;
-                                                           do (te2, ef2) <- type_check_expr Gamma Sigma e2;
+                                          | e1 :: e2 :: nil => do (te1, ef1) <- type_check_expr cenv Gamma Sigma e1;
+                                                           do (te2, ef2) <- type_check_expr cenv Gamma Sigma e2;
                                                            if (eq_type te1 te2 && (is_primint te1 || is_primlong te1) && eq_effect ef1 ef2 && eq_type te1 t) 
                                                            then OK(te1, ef1)
                                                            else Error (msg "Wrong argument types to xor operator, it expects int or long as argument")
                                           | _ =>  Error (msg "Wrong number of arguments to Binary operators") 
                                           end
                             | Cop.Oshl => match es with 
-                                          | e1 :: e2 :: nil => do (te1, ef1) <- type_check_expr Gamma Sigma e1;
-                                                           do (te2, ef2) <- type_check_expr Gamma Sigma e2;
+                                          | e1 :: e2 :: nil => do (te1, ef1) <- type_check_expr cenv Gamma Sigma e1;
+                                                           do (te2, ef2) <- type_check_expr cenv Gamma Sigma e2;
                                                            if (eq_type te1 te2 && (is_primint te1 || is_primlong te1) && eq_effect ef1 ef2 && eq_type te1 t) 
                                                            then OK(te1, ef1)
                                                            else Error (msg "Wrong argument types to shl operator, it expects int or long as argument")
                                           | _ =>  Error (msg "Wrong number of arguments to Binary operators") 
                                           end
                             | Cop.Oshr => match es with 
-                                          | e1 :: e2 :: nil => do (te1, ef1) <- type_check_expr Gamma Sigma e1;
-                                                           do (te2, ef2) <- type_check_expr Gamma Sigma e2;
+                                          | e1 :: e2 :: nil => do (te1, ef1) <- type_check_expr cenv Gamma Sigma e1;
+                                                           do (te2, ef2) <- type_check_expr cenv Gamma Sigma e2;
                                                            if (eq_type te1 te2 && (is_primint te1 || is_primlong te1) && eq_effect ef1 ef2 && eq_type te1 t) 
                                                            then OK(te1, ef1)
                                                            else Error (msg "Wrong argument types to shr operator, it expects int or long as argument")
                                           | _ =>  Error (msg "Wrong number of arguments to Binary operators") 
                                           end
                             | Cop.Oeq => match es with 
-                                          | e1 :: e2 :: nil => do (te1, ef1) <- type_check_expr Gamma Sigma e1;
-                                                               do (te2, ef2) <- type_check_expr Gamma Sigma e2;
+                                          | e1 :: e2 :: nil => do (te1, ef1) <- type_check_expr cenv Gamma Sigma e1;
+                                                               do (te2, ef2) <- type_check_expr cenv Gamma Sigma e2;
                                                                if (eq_type te1 te2 && (is_primint te1 || is_primlong te1 || is_primbool te2) && eq_effect ef1 ef2 && eq_type te1 t) 
                                                                then OK(Ptype Tbool, ef1)
                                                                else Error (msg "Wrong argument types to eq operator, it expects int or long as argument")
                                           | _ =>  Error (msg "Wrong number of arguments to Binary operators") 
                                           end
                             | Cop.One => match es with 
-                                          | e1 :: e2 :: nil => do (te1, ef1) <- type_check_expr Gamma Sigma e1;
-                                                               do (te2, ef2) <- type_check_expr Gamma Sigma e2;
+                                          | e1 :: e2 :: nil => do (te1, ef1) <- type_check_expr cenv Gamma Sigma e1;
+                                                               do (te2, ef2) <- type_check_expr cenv Gamma Sigma e2;
                                                                if (eq_type te1 te2 && (is_primint te1 || is_primlong te1 || is_primbool te2) && eq_effect ef1 ef2 && eq_type te1 t) 
                                                                then OK(Ptype Tbool, ef1)
                                                                else Error (msg "Wrong argument types to ne operator, it expects int or long as argument")
                                           | _ =>  Error (msg "Wrong number of arguments to Binary operators") 
                                           end
                             | Cop.Olt => match es with 
-                                          | e1 :: e2 :: nil => do (te1, ef1) <- type_check_expr Gamma Sigma e1;
-                                                               do (te2, ef2) <- type_check_expr Gamma Sigma e2;
+                                          | e1 :: e2 :: nil => do (te1, ef1) <- type_check_expr cenv Gamma Sigma e1;
+                                                               do (te2, ef2) <- type_check_expr cenv Gamma Sigma e2;
                                                                if (eq_type te1 te2 && (is_primint te1 || is_primlong te1) && eq_effect ef1 ef2 && eq_type te1 t) 
                                                                then OK(Ptype Tbool, ef1)
                                                                else Error (msg "Wrong argument types to lt operator, it expects int or long as argument")
                                           | _ =>  Error (msg "Wrong number of arguments to Binary operators") 
                                           end
                             | Cop.Ogt => match es with 
-                                          | e1 :: e2 :: nil => do (te1, ef1) <- type_check_expr Gamma Sigma e1;
-                                                               do (te2, ef2) <- type_check_expr Gamma Sigma e2;
+                                          | e1 :: e2 :: nil => do (te1, ef1) <- type_check_expr cenv Gamma Sigma e1;
+                                                               do (te2, ef2) <- type_check_expr cenv Gamma Sigma e2;
                                                                if (eq_type te1 te2 && (is_primint te1 || is_primlong te1) && eq_effect ef1 ef2 && eq_type te1 t) 
                                                                then OK(Ptype Tbool, ef1)
                                                                else Error (msg "Wrong argument types to gt operator, it expects int or long as argument")
                                           | _ =>  Error (msg "Wrong number of arguments to Binary operators") 
                                           end
                             | Cop.Ole => match es with 
-                                          | e1 :: e2 :: nil => do (te1, ef1) <- type_check_expr Gamma Sigma e1;
-                                                               do (te2, ef2) <- type_check_expr Gamma Sigma e2;
+                                          | e1 :: e2 :: nil => do (te1, ef1) <- type_check_expr cenv Gamma Sigma e1;
+                                                               do (te2, ef2) <- type_check_expr cenv Gamma Sigma e2;
                                                                if (eq_type te1 te2 && (is_primint te1 || is_primlong te1) && eq_effect ef1 ef2 && eq_type te1 t) 
                                                                then OK(Ptype Tbool, ef1)
                                                                else Error (msg "Wrong argument types to le operator, it expects int or long as argument")
                                           | _ =>  Error (msg "Wrong number of arguments to Binary operators") 
                                           end
                             | Cop.Oge => match es with 
-                                          | e1 :: e2 :: nil => do (te1, ef1) <- type_check_expr Gamma Sigma e1;
-                                                               do (te2, ef2) <- type_check_expr Gamma Sigma e2;
+                                          | e1 :: e2 :: nil => do (te1, ef1) <- type_check_expr cenv Gamma Sigma e1;
+                                                               do (te2, ef2) <- type_check_expr cenv Gamma Sigma e2;
                                                                if (eq_type te1 te2 && (is_primint te1 || is_primlong te1) && eq_effect ef1 ef2 && eq_type te1 t) 
                                                                then OK(Ptype Tbool, ef1)
                                                                else Error (msg "Wrong argument types to ge operator, it expects int or long as argument")
@@ -253,14 +285,14 @@ match e with
                             end
                  | Run h => Error (msg "Run is not yet supported")
                  end
-| Bind x t e1 e2 t' => do (te1, ef1) <- type_check_expr Gamma Sigma e1;
-                       do (te2, ef2) <- type_check_expr (extend_context Gamma x t) Sigma e2;
+| Bind x t e1 e2 t' => do (te1, ef1) <- type_check_expr cenv Gamma Sigma e1;
+                       do (te2, ef2) <- type_check_expr cenv (extend_context Gamma x t) Sigma e2;
                        if eq_type te2 t'
                        then OK (te2, ef1 ++ ef2)
                        else Error (msg "Type of bind does not match the inferred type")
-| Cond e1 e2 e3 t =>  do (te1, ef1) <- type_check_expr Gamma Sigma e1;
-                      do (te2, ef2) <- type_check_expr Gamma Sigma e2;
-                      do (te3, ef3) <- type_check_expr Gamma Sigma e3;
+| Cond e1 e2 e3 t =>  do (te1, ef1) <- type_check_expr cenv Gamma Sigma e1;
+                      do (te2, ef2) <- type_check_expr cenv Gamma Sigma e2;
+                      do (te3, ef3) <- type_check_expr cenv Gamma Sigma e3;
                       if is_primbool te1 && eq_type te2 te3 && eq_effect ef2 ef3 && eq_type t te2
                       then OK (te1, ef1 ++ ef2)
                       else Error (msg "Type of cond does not match the inferred type")
@@ -274,21 +306,47 @@ match e with
                    end
 | Hexpr h e t =>  Error (msg "Hexpr is not yet supported")
 | Eapp ef ts es t => Error (msg "Not found") (* we need to check with the map that contains all external call info *)
+| Sfield e x t => do (te, ef) <- type_check_expr cenv Gamma Sigma e;
+                  match te with 
+                  | Stype id a => match cenv!id with 
+                                  | Some co => do ct <- type_of_member a x (bmembers_cmembers co.(co_members));
+                                               do bt <- trans_ctype_btype ct;
+                                               if eq_type t bt 
+                                               then OK (te, nil)
+                                               else Error (msg "Wrong type inferred for the struct field")
+                                  | None => Error (msg "Struct information not found in composite env")
+                                  end
+                  | _ => Error (msg "Should be a struct type")
+                  end
 end.
 
 Open Scope string_scope.
 
-Definition type_check_function (Gamma : ty_context) (Sigma : store_context) (fn : function) : res string :=
-match type_check_expr Gamma Sigma fn.(fn_body) with 
+Fixpoint bind_vars (Gamma : ty_context) (l: list (ident * type)) : ty_context :=
+match l with
+| nil => Gamma
+| (id, ty) :: l => bind_vars (PTree.set id ty Gamma) l
+end.
+
+Fixpoint bind_globdef (Gamma: ty_context) (l: list (ident * globdef fundef type)) : ty_context :=
+match l with
+| nil => Gamma
+| (id, Gfun fd) :: l => bind_globdef (PTree.set id (type_of_fundef fd) Gamma) l
+| (id, Gvar v) :: l => bind_globdef (PTree.set id v.(gvar_info) Gamma) l
+end.
+
+Definition type_check_function (cenv : bcomposite_env) (Gamma : ty_context) (Sigma : store_context) (fn : function) : res string :=
+let Gamma' := bind_vars (bind_vars Gamma fn.(fn_args)) fn.(fn_vars) in
+match type_check_expr cenv Gamma' Sigma fn.(fn_body) with 
 | Error msg => Error msg
 | OK tef => if eq_type fn.(fn_return) tef.1 && eq_effect fn.(fn_effect) tef.2
              then OK "Success in type checking" 
              else Error (msg "Type of function body does not match with the return type in the function declaration")
 end.
 
-Definition type_check_fundef (Gamma : ty_context) (Sigma : store_context) (fn : BeePL.fundef) : res string :=
+Definition type_check_fundef (cenv : bcomposite_env) (Gamma : ty_context) (Sigma : store_context) (fn : BeePL.fundef) : res string :=
 match fn with 
-| Internal f => type_check_function Gamma Sigma f 
+| Internal f => type_check_function cenv Gamma Sigma f 
 | External ef ts t cc => match ef with 
                          | EF_external fn fs => if eq_types eq_type fs.(bsig_args) ts && eq_type t fs.(bsig_res) (* add the check with the map *)
                                                 then OK "Success in type checking" 
@@ -302,28 +360,29 @@ OK (gv.(gvar_info)).
 
 Section Type_check_globdefs.
 
-Variable type_check_globdef : ty_context -> store_context -> BeePL.globdef BeePL.fundef BeeTypes.type -> res string.
+Variable type_check_globdef : bcomposite_env -> ty_context -> store_context -> BeePL.globdef BeePL.fundef BeeTypes.type -> res string.
 
-Fixpoint type_check_globdefs (Gamma : ty_context) (Sigma : store_context) (gds : list (BeePL.globdef BeePL.fundef BeeTypes.type)) : res string :=
+Fixpoint type_check_globdefs (cenv : bcomposite_env) (Gamma : ty_context) (Sigma : store_context) (gds : list (BeePL.globdef BeePL.fundef BeeTypes.type)) : res string :=
 match gds with 
 | nil => OK "Program type checks!"
-| gd :: gds => do gds1 <- type_check_globdef Gamma Sigma gd;
-               type_check_globdefs Gamma Sigma gds
+| gd :: gds => do gds1 <- type_check_globdef cenv Gamma Sigma gd;
+               type_check_globdefs cenv Gamma Sigma gds
 end.
   
 End Type_check_globdefs.
 
-Definition type_check_globdef (Gamma : ty_context) (Sigma : store_context)  (gd : BeePL.globdef BeePL.fundef BeeTypes.type) : res string :=
+Definition type_check_globdef (cenv : bcomposite_env) (Gamma : ty_context) (Sigma : store_context)  (gd : BeePL.globdef BeePL.fundef BeeTypes.type) : res string :=
 match gd with 
-| AST.Gfun f => type_check_fundef Gamma Sigma f  
+| AST.Gfun f => type_check_fundef cenv Gamma Sigma f  
 | Gvar g => do gt <- type_check_globvar Gamma Sigma g;
             OK "Success in type checking globdef"
 end.
 
-(* Add later type checking for composite definitions *)
-Definition type_check_program (Gamma : ty_context) (Sigma : store_context) (p : BeePL.program) : res string :=
-type_check_globdefs type_check_globdef Gamma Sigma (unzip2 (p.(prog_defs))).
-
+(* Fix Store context: How to compute this? *)
+Definition type_check_program (p : BeePL.program) : res string :=
+let Gamma := bind_globdef (PTree.empty _) p.(prog_defs) in
+let cenv := p.(prog_comp_env) in 
+type_check_globdefs type_check_globdef cenv Gamma empty_context (unzip2 (p.(prog_defs))).
 
 
 
