compiler_test/beepl_test/BeePL_progs.v
@@ -1,8 +1,9 @@
+
 Require Import AST Maps Ctypes.
-Require Import BeePL BeeTypes Errors BeePL_typechecker. 
+Require Import BeePL BeeTypes Errors BeePL_typechecker Csyntaxdefs. 
 From Coq Require Import String.
 
-Require Import BeePL_add BeePL_cond BeePL_app BeePL_div_zero.
+Require Import BeePL_add BeePL_cond BeePL_app BeePL_div_zero BeePL_struct_ex1.
 
 (* In this file you will see two definitions. One for example1 and the other for
    example1_atom_of_string. Those two definitions are extracted to OCaml by 
@@ -21,21 +22,35 @@ Require Import BeePL_add BeePL_cond BeePL_app BeePL_div_zero.
 
 (* Construct the BeePL.program *)
 
-Definition composites : list composite_definition := nil.
+Definition bcomposites : list bcomposite_definition := nil.
 
-Lemma composite_default :
-  build_composite_env nil = OK (PTree.empty composite).
+Lemma bcomposite_default :
+  wf_bcomposites bcomposites.
 Proof.
-  unfold build_composite_env; simpl; reflexivity.
+  unfold wf_bcomposites.
+  unfold build_bcomposite_env; simpl; reflexivity.
 Qed.
+*Definition example1 : BeePL.program := @mkbprogram bcomposites 
+                                                   BeePL_add.global_definitions 
+                                                   BeePL_add.public_idents 
+                                                   BeePL_add._main 
+                                                   bcomposite_default.
 
-Definition example1 : BeePL.program := {| prog_defs := BeePL_div_zero.global_definitions; (* <-- MODIFY *)
-                                          prog_public := BeePL_div_zero.public_idents;    (* <-- MODIFY *)
-                                          prog_main := BeePL_div_zero._main;              (* <-- MODIFY *)
+(*Definition example1 : BeePL.program := @mkbprogram BeePL_struct_ex1.bcomposites 
+                                                   BeePL_struct_ex1.global_definitions 
+                                                   BeePL_struct_ex1.public_idents 
+                                                   BeePL_struct_ex1._main 
+                                                   BeePL_struct_ex1.bcomposite_correct.*)
+
+(*Definition example1 : BeePL.program := {| prog_defs := BeePL_add.global_definitions; (* <-- MODIFY *)
+                                          prog_public := BeePL_add.public_idents;    (* <-- MODIFY *)
+                                          prog_main := BeePL_add._main;              (* <-- MODIFY *)
                                           prog_types := composites;
-                                          prog_comp_env := PTree.empty composite;
-                                          prog_comp_env_eq := composite_default |}.
+                                          prog_comp_env := PTree.empty bcomposite;
+                                          prog_comp_env_eq := bcomposite_default |}.*)
 
-Definition example1_atom_of_string : list (ident * string) := BeePL_div_zero.atom_of_string. (* <-- MODIFY *)
 
-Compute (type_check_program empty_context empty_context example1).
+Definition example1_atom_of_string : list (ident * string) := BeePL_struct_ex1.atom_of_string. (* <-- MODIFY *)
+
+Compute (type_check_program example1).
+
