beepl/BeePL_values.v
@@ -208,4 +208,5 @@ match t with
              end
 | Reftype h b a => error (msg "Tpointer not allowed")
 | Ftype ts e t => error (msg "Tfunction not allowed")
+| Stype x a => error (msg "Struct not allowed")
 end.
