compiler_test/beepl_test/BeePL_struct_ex1.v
@@ -1,0 +1,196 @@
+Require Import Integers AST Ctypes BeePL BeeTypes BeePL_values BeePL_typechecker BeePL_Csyntax. 
+From Coq Require Import String ZArith Lists.List.
+From compcert Require Import Csyntaxdefs Errors Maps BeePL_aux.
+Import Csyntaxdefs.CsyntaxNotations.
+Local Open Scope string_scope.
+Local Open Scope csyntax_scope.
+
+(* #include <stdio.h>
+
+// Define a struct to represent a point in 2D
+struct Point {
+    int x;
+    int y;
+};
+
+int main() {
+    struct Point p1;       // Declare a variable of type struct Point
+    p1.x = 10;             // Assign values to fields
+    p1.y = 20;
+    return p1.x;
+}*)
+
+(* attr_alignas is optional *)
+Definition dattr := {| attr_volatile := false; attr_alignas := None |}.
+Definition _Point : ident := $"Point".
+Definition _p1 : ident := $"p1".
+Definition _x : ident := $"x".
+Definition _y : ident := $"y".
+Definition _x1 : ident := $"_x1".
+Definition _y1 : ident := $"_y1".
+Definition _main : ident := $"main".
+
+Definition atom_of_string : list (ident * string) := ((_Point, "Point") ::
+                                                      (_p1, "p1") ::
+                                                      (_x, "x") :: 
+                                                      (_y, "y") :: 
+                                                      (_x1, "x1") ::
+                                                      (_y1, "y1") :: 
+                                                      (_main, "main") :: nil).
+Definition f_struct : BeePL.function := {| 
+                                   fn_return := (Ptype (BeeTypes.Tint I32 Unsigned dattr));
+                                   fn_effect := nil;
+                                   fn_callconv := cc_default;
+                                   fn_args := nil;
+                                   fn_vars := ((_p1, BeeTypes.Stype _Point dattr) :: nil);
+                                   fn_body := Bind 
+                                                (_p1) 
+                                                (BeeTypes.Stype _Point dattr)
+                                                (Unit (Ptype Tunit))
+                                                (Bind 
+                                                   (_x1)
+                                                   (BeeTypes.Ptype (BeeTypes.Tint Ctypes.I32 Ctypes.Unsigned dattr))
+                                                   (Sfield (Var _p1 (BeeTypes.Stype _Point dattr)) _x 
+                                                           (BeeTypes.Ptype (BeeTypes.Tint Ctypes.I32 Ctypes.Unsigned dattr)))
+                                                   (Bind 
+                                                      (_x1)
+                                                      (BeeTypes.Ptype (BeeTypes.Tint Ctypes.I32 Ctypes.Unsigned dattr))
+                                                      (Const (ConsInt (Int.repr 10)) (Ptype (BeeTypes.Tint I32 Signed dattr)))
+                                                      (Bind 
+                                                         (_y1)
+                                                         (BeeTypes.Ptype (BeeTypes.Tint Ctypes.I32 Ctypes.Unsigned dattr))
+                                                         (Sfield (Var _p1 (BeeTypes.Stype _Point dattr)) _y 
+                                                                 (BeeTypes.Ptype (BeeTypes.Tint Ctypes.I32 Ctypes.Unsigned dattr)))
+                                                         (Bind 
+                                                            (_y1)
+                                                            (BeeTypes.Ptype (BeeTypes.Tint Ctypes.I32 Ctypes.Unsigned dattr))
+                                                            (Const (ConsInt (Int.repr 20)) (Ptype (BeeTypes.Tint I32 Signed dattr)))
+                                                            (Var _x1 (BeeTypes.Ptype (BeeTypes.Tint Ctypes.I32 Ctypes.Unsigned dattr)))
+                                                            (BeeTypes.Ptype (BeeTypes.Tint Ctypes.I32 Ctypes.Unsigned dattr)))
+                                                         (BeeTypes.Ptype (BeeTypes.Tint Ctypes.I32 Ctypes.Unsigned dattr)))
+                                                   (BeeTypes.Ptype (BeeTypes.Tint Ctypes.I32 Ctypes.Unsigned dattr)))
+                                                (BeeTypes.Ptype (BeeTypes.Tint Ctypes.I32 Ctypes.Unsigned dattr)))
+                                               (BeeTypes.Ptype (BeeTypes.Tint Ctypes.I32 Ctypes.Unsigned dattr))
+                                                   
+                                                    |}.
+
+Definition global_definitions : list (ident * AST.globdef BeePL.fundef type) 
+   := (_main, AST.Gfun(BeePL.Internal (f_struct))) :: nil.
+
+Definition public_idents : list ident := (_main :: nil).
+
+Definition bcomposites : list bcomposite_definition :=
+(Bcomposite _Point Struct
+   (Member_plain _x (BeeTypes.Ptype (BeeTypes.Tint Ctypes.I32 Ctypes.Unsigned dattr)) :: 
+    Member_plain _y (BeeTypes.Ptype (BeeTypes.Tint Ctypes.I32 Ctypes.Unsigned dattr)) :: nil)
+   noattr :: nil).
+
+Lemma bcomposite_correct :
+  wf_bcomposites bcomposites.
+Proof.
+  unfold wf_bcomposites.
+  unfold build_bcomposite_env; simpl; constructor. 
+Qed.
+
+(*Definition example1 : BeePL.program := @mkbprogram bcomposites global_definitions public_idents _main bcomposite_correct.
+
+Compute (type_check_program example1). (* debug why typecheck fails *)
+
+Compute (BeePL_Csyntax.BeePL_compcert example1).*)
+
+(*  = OK
+         {|
+           Ctypes.prog_defs :=
+             (22880918%positive,
+             Gfun
+               (Ctypes.Internal
+                  {|
+                    Csyntax.fn_return := Ctypes.Tint I32 Unsigned {| attr_volatile := false; attr_alignas := None |};
+                    Csyntax.fn_callconv := {| cc_vararg := None; cc_unproto := false; cc_structret := false |};
+                    Csyntax.fn_params := nil;
+                    Csyntax.fn_vars :=
+                      (4185%positive, Tstruct 1566385715%positive {| attr_volatile := false; attr_alignas := None |}) :: nil;
+                    Csyntax.fn_body :=
+                      Csyntax.Ssequence
+                        (Csyntax.Sdo
+                           (Csyntax.Eassign
+                              (Csyntax.Evar 4185%positive
+                                 (Tstruct 1566385715%positive {| attr_volatile := false; attr_alignas := None |}))
+                              (Csyntax.Eval (Values.Vint {| Int.intval := 0; Int.intrange := Int.Z_mod_modulus_range' 0 |}) Tvoid)
+                              Tvoid))
+                        (Csyntax.Ssequence
+                           (Csyntax.Sdo
+                              (Csyntax.Eassign
+                                 (Csyntax.Evar 268414%positive
+                                    (Ctypes.Tint I32 Unsigned {| attr_volatile := false; attr_alignas := None |}))
+                                 (Csyntax.Efield
+                                    (Csyntax.Evar 4185%positive
+                                       (Tstruct 1566385715%positive {| attr_volatile := false; attr_alignas := None |}))
+                                    97%positive (Ctypes.Tint I32 Unsigned {| attr_volatile := false; attr_alignas := None |}))
+                                 Tvoid))
+                           (Csyntax.Ssequence
+                              (Csyntax.Sdo
+                                 (Csyntax.Eassign
+                                    (Csyntax.Evar 268414%positive
+                                       (Ctypes.Tint I32 Unsigned {| attr_volatile := false; attr_alignas := None |}))
+                                    (Csyntax.Eval
+                                       (Values.Vint {| Int.intval := 10; Int.intrange := Int.Z_mod_modulus_range' 10 |})
+                                       (Ctypes.Tint I32 Signed {| attr_volatile := false; attr_alignas := None |})) Tvoid))
+                              (Csyntax.Ssequence
+                                 (Csyntax.Sdo
+                                    (Csyntax.Eassign
+                                       (Csyntax.Evar 268478%positive
+                                          (Ctypes.Tint I32 Unsigned {| attr_volatile := false; attr_alignas := None |}))
+                                       (Csyntax.Efield
+                                          (Csyntax.Evar 4185%positive
+                                             (Tstruct 1566385715%positive {| attr_volatile := false; attr_alignas := None |}))
+                                          98%positive
+                                          (Ctypes.Tint I32 Unsigned {| attr_volatile := false; attr_alignas := None |})) Tvoid))
+                                 (Csyntax.Ssequence
+                                    (Csyntax.Sdo
+                                       (Csyntax.Eassign
+                                          (Csyntax.Evar 268478%positive
+                                             (Ctypes.Tint I32 Unsigned {| attr_volatile := false; attr_alignas := None |}))
+                                          (Csyntax.Eval
+                                             (Values.Vint {| Int.intval := 20; Int.intrange := Int.Z_mod_modulus_range' 20 |})
+                                             (Ctypes.Tint I32 Signed {| attr_volatile := false; attr_alignas := None |})) Tvoid))
+                                    (Csyntax.Sreturn
+                                       (Some
+                                          (Csyntax.Evalof
+                                             (Csyntax.Evar 268414%positive
+                                                (Ctypes.Tint I32 Unsigned {| attr_volatile := false; attr_alignas := None |}))
+                                             (Ctypes.Tint I32 Unsigned {| attr_volatile := false; attr_alignas := None |}))))))))
+                  |})) :: nil;
+           Ctypes.prog_public := 22880918%positive :: nil;
+           Ctypes.prog_main := 22880918%positive;
+           Ctypes.prog_types :=
+             Composite 1566385715%positive Struct
+               (Ctypes.Member_plain 97%positive (Ctypes.Tint I32 Unsigned {| attr_volatile := false; attr_alignas := None |})
+                :: Ctypes.Member_plain 98%positive (Ctypes.Tint I32 Unsigned {| attr_volatile := false; attr_alignas := None |})
+                   :: nil) {| attr_volatile := false; attr_alignas := None |} :: nil;
+           Ctypes.prog_comp_env :=
+             PTree.Nodes
+               (PTree.Node001
+                  (PTree.Node001
+                     (PTree.Node100
+                        (PTree.Node100
+                           (PTree.Node001
+                              (PTree.Node001
+                                 (PTree.Node100
+                                    (PTree.Node100
+                                       (PTree.Node100
+                                          (PTree.Node001
+                                             (PTree.Node001
+                                                (PTree.Node100
+                                                   (PTree.Node100
+                                                      (PTree.Node001
+                                                         (PTree.Node100
+                                                            (PTree.Node100
+                                                               (PTree.Node001
+                                                                  (PTree.Node100
+                                                                     (PTree.Node001 (PTree.Node001 (PTree.Node001 ...)))))))))))))))))))));
+           Ctypes.prog_comp_env_eq := eq_refl
+         |}
+     : res (Ctypes.program Csyntax.function)
+*)
+
